Clap/Sha2/Test.lean
@@ -8,21 +8,21 @@ open Clap.Sha2
 
 def stringToU8s (s:String) : Array UInt8 := s.toUTF8.data
 
-example : digest (t := Clap.Sha2.Cpu.t) (stringToU8s "abc") =
-  some #[0xba7816bf, 0x8f01cfea, 0x414140de, 0x5dae2223, 0xb00361a3, 0x96177a9c, 0xb410ff61, 0xf20015ad] := by
+example : Id.run (digest Id (t := Clap.Sha2.Cpu.t) (stringToU8s "abc")) =
+  #[0xba7816bf, 0x8f01cfea, 0x414140de, 0x5dae2223, 0xb00361a3, 0x96177a9c, 0xb410ff61, 0xf20015ad] := by
   native_decide
 
-example : digest (t := Clap.Sha2.Cpu.t) (stringToU8s "abcdbcdecdefdefgefghfghighijhijkijkljklmklmnlmnomnopnopq") =
-  some #[0x248d6a61, 0xd20638b8, 0xe5c02693, 0x0c3e6039, 0xa33ce459, 0x64ff2167, 0xf6ecedd4, 0x19db06c1] := by
+example : Id.run (digest Id (t := Clap.Sha2.Cpu.t) (stringToU8s "abcdbcdecdefdefgefghfghighijhijkijkljklmklmnlmnomnopnopq")) =
+  #[0x248d6a61, 0xd20638b8, 0xe5c02693, 0x0c3e6039, 0xa33ce459, 0x64ff2167, 0xf6ecedd4, 0x19db06c1] := by
   native_decide
 
 end TestCpu
-/-
+
 namespace TestCircuit
 
 abbrev p := Primes.goldilocks
 
-open Clap.Sha2
+open Clap.Sha2 Circuit
 open Clap.Lang Core ZMod
 
 def stringToU8s (s:String) : Array (F8 p) :=
@@ -31,10 +31,14 @@ def stringToU8s (s:String) : Array (F8 p) :=
     let b : F p := (b.toNat : F p)
     F8.ofF! b
 
-example : digest (t := Clap.Sha2.Circuit.t p) (stringToU8s "abc") = #[0xba7816bf, 0x8f01cfea, 0x414140de, 0x5dae2223, 0xb00361a3, 0x96177a9c, 0xb410ff61, 0xf20015ad] := by native_decide
+private instance : Sha Option (t p) := Clap.Sha2.Circuit.instShaOptionT
 
-example : digest (t := Clap.Sha2.Circuit.t p) (stringToU8s "abcdbcdecdefdefgefghfghighijhijkijkljklmklmnlmnomnopnopq") =
-   #[0x248d6a61, 0xd20638b8, 0xe5c02693, 0x0c3e6039, 0xa33ce459, 0x64ff2167, 0xf6ecedd4, 0x19db06c1] := by native_decide
+example : digest Option (t := Clap.Sha2.Circuit.t p) (stringToU8s "abc") =
+  some #[0xba7816bf, 0x8f01cfea, 0x414140de, 0x5dae2223, 0xb00361a3, 0x96177a9c, 0xb410ff61, 0xf20015ad] := by
+  native_decide
+
+example : digest Option (t := Clap.Sha2.Circuit.t p) (stringToU8s "abcdbcdecdefdefgefghfghighijhijkijkljklmklmnlmnomnopnopq") =
+  some #[0x248d6a61, 0xd20638b8, 0xe5c02693, 0x0c3e6039, 0xa33ce459, 0x64ff2167, 0xf6ecedd4, 0x19db06c1] := by
+  native_decide
 
 end TestCircuit
--/
